code/bignum/Hacl.Bignum.SafeAPI.fst
@@ -138,13 +138,13 @@ let bn_mod_slow_safe_st (t:limb_t) (len:BN.meta_len t) =
 inline_for_extraction noextract
 val bn_mod_slow_safe:
     #t:limb_t
-  -> #len:BN.meta_len t
-  -> k:BM.mont t len
-  -> bn_check_bn_mod:BR.bn_check_bn_mod_st t len
-  -> bn_mod_slow_precompr2:BR.bn_mod_slow_precompr2_st t len ->
-  bn_mod_slow_safe_st t len
+  -> k:BM.mont t
+  -> bn_check_bn_mod:BR.bn_check_bn_mod_st t k.BM.bn.BN.len
+  -> bn_mod_slow_precompr2:BR.bn_mod_slow_precompr2_st t k.BM.bn.BN.len ->
+  bn_mod_slow_safe_st t k.BM.bn.BN.len
 
-let bn_mod_slow_safe #t #len k bn_check_bn_mod bn_mod_slow_safe_st n a res =
+let bn_mod_slow_safe #t k bn_check_bn_mod bn_mod_slow_safe_st n a res =
+  [@inline_let] let len = k.BM.bn.BN.len in
   let h0 = ST.get () in
   let is_valid_m = bn_check_bn_mod n a in
   BR.bn_mod_slow k bn_mod_slow_safe_st n a res;
@@ -178,16 +178,16 @@ let bn_mod_exp_safe_st (t:limb_t) (len:BN.meta_len t) =
 inline_for_extraction noextract
 val bn_mod_exp_safe:
     #t:limb_t
-  -> #len:BN.meta_len t
-  -> k:BM.mont t len
-  -> bn_check_mod_exp:BE.bn_check_mod_exp_st t len
-  -> bn_mod_exp_precompr2:BE.bn_mod_exp_precompr2_st t len ->
-  bn_mod_exp_safe_st t len
+  -> k:BM.mont t
+  -> bn_check_mod_exp:BE.bn_check_mod_exp_st t k.BM.bn.BN.len
+  -> bn_mod_exp_precompr2:BE.bn_mod_exp_precompr2_st t k.BM.bn.BN.len ->
+  bn_mod_exp_safe_st t k.BM.bn.BN.len
 
-let bn_mod_exp_safe #t #len k bn_check_mod_exp bn_mod_exp_precompr2 n a bBits b res =
+let bn_mod_exp_safe #t k bn_check_mod_exp bn_mod_exp_precompr2 n a bBits b res =
+  [@inline_let] let len = k.BM.bn.BN.len in
   let h0 = ST.get () in
   let is_valid_m = bn_check_mod_exp n a bBits b in
-  BE.bn_mod_exp #t #len k bn_mod_exp_precompr2 n a bBits b res;
+  BE.bn_mod_exp #t k bn_mod_exp_precompr2 n a bBits b res;
   let h1 = ST.get () in
   mapT len res (logand is_valid_m) res;
   let h2 = ST.get () in
@@ -202,16 +202,16 @@ let bn_mod_exp_safe #t #len k bn_check_mod_exp bn_mod_exp_precompr2 n a bBits b 
 inline_for_extraction noextract
 val bn_mod_exp_mont_ladder_safe:
     #t:limb_t
-  -> #len:BN.meta_len t
-  -> k:BM.mont t len
-  -> bn_check_mod_exp:BE.bn_check_mod_exp_st t len
-  -> bn_mod_exp_mont_ladder_precompr2:BE.bn_mod_exp_mont_ladder_precompr2_st t len ->
-  bn_mod_exp_safe_st t len
+  -> k:BM.mont t
+  -> bn_check_mod_exp:BE.bn_check_mod_exp_st t k.BM.bn.BN.len
+  -> bn_mod_exp_mont_ladder_precompr2:BE.bn_mod_exp_mont_ladder_precompr2_st t k.BM.bn.BN.len ->
+  bn_mod_exp_safe_st t k.BM.bn.BN.len
 
-let bn_mod_exp_mont_ladder_safe #t #len k bn_check_mod_exp bn_mod_exp_mont_ladder_precompr2 n a bBits b res =
+let bn_mod_exp_mont_ladder_safe #t k bn_check_mod_exp bn_mod_exp_mont_ladder_precompr2 n a bBits b res =
+  [@inline_let] let len = k.BM.bn.BN.len in
   let h0 = ST.get () in
   let is_valid_m = bn_check_mod_exp n a bBits b in
-  BE.bn_mod_exp_mont_ladder #t #len k bn_mod_exp_mont_ladder_precompr2 n a bBits b res;
+  BE.bn_mod_exp_mont_ladder #t k bn_mod_exp_mont_ladder_precompr2 n a bBits b res;
   let h1 = ST.get () in
   mapT len res (logand is_valid_m) res;
   let h2 = ST.get () in
